Unary logical relations

stlc/logrel.v
@@ -1,70 +1,212 @@
 From iris.program_logic Require Export weakestpre.
 From iris.proofmode Require Export tactics.
 From stlc Require Export lang typing.
+From iris.algebra Require Import list.
+From iris.base_logic Require Import invariants.
+Import uPred.
 
 Reserved Notation "⟦ τ ⟧" (at level 0, τ at level 70).
 Reserved Notation "⟦ τ ⟧ₑ" (at level 0, τ at level 70).
 Reserved Notation "⟦ Γ ⟧*" (at level 0, Γ at level 70).
 
+
 (** interp : is a unary logical relation. *)
 Section logrel.
-Context `{irisG stlc_lang Σ}.
+Context `{LANG: irisG stlc_lang Σ}.
+  Notation D := (valO stlc_lang -n> iPropO Σ).
+  Implicit Types τi : D.
+  Implicit Types Δ : listO D.
+  Implicit Types interp : listO D → D.
 
-Fixpoint interp (τ : type) (w : val) : iProp Σ :=
-  match τ with
-  | TUnit => ⌜w = UnitV⌝
-  | TProd τ1 τ2 => ∃ w1 w2, ⌜w = PairV w1 w2⌝ ∧ ⟦ τ1 ⟧ w1 ∧ ⟦ τ2 ⟧ w2
-  | TSum τ1 τ2 =>
-     (∃ w1, ⌜w = InjLV w1⌝ ∧ ⟦ τ1 ⟧ w1) ∨ (∃ w2, ⌜w = InjRV w2⌝ ∧ ⟦ τ2 ⟧ w2)
-  | TArrow τ1 τ2 => □ ∀ v, ⟦ τ1 ⟧ v → WP App (# w) (# v) {{ ⟦ τ2 ⟧ }}
-  end%I
-where "⟦ τ ⟧" := (interp τ).
+  Program Definition env_lookup (x : var) : listO D -n> D := λne Δ,
+    from_option id (cconst True)%I (Δ !! x).
+  Solve Obligations with solve_proper.
 
-Definition interp_expr (τ : type) (e : expr) : iProp Σ :=
-  WP e {{ ⟦ τ ⟧ }}%I.
+  Program Definition interp_unit : listO D -n> D.
+    refine (λne Δ w, ⌜w = _⌝%I). Unshelve. 2 : exact UnitV.
+    red. repeat intro; eauto.
+    red. repeat intro; eauto. repeat red in H. subst; auto.
+  Defined.
 
-Global Instance interp_persistent τ v : Persistent (⟦ τ ⟧ v).
-Proof. revert v; induction τ=> v /=; apply _. Qed.
+  Program Definition interp_prod
+      (interp1 interp2 : listO D -n> D) : listO D -n> D := λne Δ w,
+    (∃ w1 w2, ⌜w = PairV w1 w2⌝ ∧ interp1 Δ w1 ∧ interp2 Δ w2)%I.
+  Solve Obligations with repeat intros ?; simpl; solve_proper.
 
-Global Instance interp_env_base_persistent Γ vs :
-  TCForall Persistent (zip_with (λ τ, ⟦ τ ⟧) Γ vs).
-Proof.
-  revert vs; induction Γ => vs; simpl; destruct vs; constructor; apply _.
-Qed.
+  Program Definition interp_sum
+      (interp1 interp2 : listO D -n> D) : listO D -n> D := λne Δ w,
+    ((∃ w1, ⌜w = InjLV w1⌝ ∧ interp1 Δ w1) ∨ (∃ w2, ⌜w = InjRV w2⌝ ∧ interp2 Δ w2))%I.
+  Solve Obligations with repeat intros ?; simpl; solve_proper.
 
-Definition interp_env (Γ : list type) (vs : list val) : iProp Σ :=
-  (⌜length Γ = length vs⌝ ∗ [∗] zip_with (λ τ, ⟦ τ ⟧) Γ vs)%I.
+  Program Definition interp_arrow
+      (interp1 interp2 : listO D -n> D) : listO D -n> D := λne Δ w,
+    (□ ∀ v, interp1 Δ v → WP App (of_val w) (of_val v) {{ interp2 Δ }})%I.
+  Solve Obligations with repeat intros ?; simpl; solve_proper.
 
-Notation "⟦ Γ ⟧*" := (interp_env Γ).
+  Program Definition interp_rec1
+      (interp : listO D -n> D) (Δ : listO D) (τi : D) : D := λne w,
+    (□ (∃ v, ⌜w = FoldV v⌝ ∧ ▷ interp (τi :: Δ) v))%I.
 
-Global Instance interp_env_persistent Γ vs :
-  Persistent (⟦ Γ ⟧* vs) := _.
+  Global Instance interp_rec1_contractive
+    (interp : listO D -n> D) (Δ : listO D) : Contractive (interp_rec1 interp Δ).
+  Proof. by solve_contractive. Qed.
 
-Lemma interp_env_nil : ⊢ ⟦ [] ⟧* [].
-Proof. iSplit; simpl; auto. Qed.
-Lemma interp_env_cons Γ vs τ v :
-    ⟦ τ :: Γ ⟧* (v :: vs) ⊣⊢ ⟦ τ ⟧ v ∗ ⟦ Γ ⟧* vs.
-  Proof.
-    rewrite /interp_env /= (assoc _ (⟦ _ ⟧ _)) -(comm _ ⌜(_ = _)⌝%I) -assoc.
-    by apply bi.sep_proper; [apply bi.pure_proper; lia|].
+  Lemma fixpoint_interp_rec1_eq (interp : listO D -n> D) Δ x :
+    fixpoint (interp_rec1 interp Δ) x ≡ interp_rec1 interp Δ (fixpoint (interp_rec1 interp Δ)) x.
+  Proof. exact: (fixpoint_unfold (interp_rec1 interp Δ) x). Qed.
+
+  Program Definition interp_rec (interp : listO D -n> D) : listO D -n> D := λne Δ,
+    fixpoint (interp_rec1 interp Δ).
+  Next Obligation.
+    intros interp n Δ1 Δ2 HΔ; apply fixpoint_ne => τi w. solve_proper.
   Qed.
 
-Lemma interp_env_length Γ vs : ⟦ Γ ⟧* vs ⊢ ⌜length Γ = length vs⌝.
-Proof. by iIntros "[% ?]". Qed.
+  Fixpoint interp (τ : type) : listO D -n> D :=
+    match τ return _ with
+    | TUnit => interp_unit
+    | TProd τ1 τ2 => interp_prod (interp τ1) (interp τ2)
+    | TVar x => env_lookup x
+    | TSum τ1 τ2 => interp_sum (interp τ1) (interp τ2)
+    | TArrow τ1 τ2 => interp_arrow (interp τ1) (interp τ2)
+    | TRec τ' => interp_rec (interp τ')
+    end.
+  Notation "⟦ τ ⟧" := (interp τ).
 
-Lemma interp_env_Some_l Γ vs x τ :
-  Γ !! x = Some τ → ⟦ Γ ⟧* vs ⊢ ∃ v, ⌜vs !! x = Some v⌝ ∧ ⟦ τ ⟧ v.
-Proof.
-  iIntros (?) "[Hlen HΓ]"; iDestruct "Hlen" as %Hlen.
-  destruct (lookup_lt_is_Some_2 vs x) as [v Hv].
-  { by rewrite -Hlen; apply lookup_lt_Some with τ. }
-  iExists v; iSplit. done. iApply (big_sepL_elem_of with "HΓ").
-  apply elem_of_list_lookup_2 with x.
-  rewrite lookup_zip_with; by simplify_option_eq.
-Qed.
+Definition interp_env (Γ : list type)
+      (Δ : listO D) (vs : list val) : iProp Σ :=
+    (⌜length Γ = length vs⌝ ∗ [∗] zip_with (λ τ, ⟦ τ ⟧ Δ) Γ vs)%I.
+  Notation "⟦ Γ ⟧*" := (interp_env Γ).
 
+  Definition interp_expr (τ : type) (Δ : listO D) (e : expr) : iProp Σ :=
+    WP e {{ ⟦ τ ⟧ Δ }}%I.
+
+  Class env_Persistent Δ :=
+    env_persistent : Forall (λ τi, ∀ v, Persistent (τi v)) Δ.
+  Global Instance env_persistent_nil : env_Persistent [].
+  Proof. by constructor. Qed.
+  Global Instance env_persistent_cons τi Δ :
+    (∀ v, Persistent (τi v)) → env_Persistent Δ → env_Persistent (τi :: Δ).
+  Proof. by constructor. Qed.
+  Global Instance env_persistent_lookup Δ x v :
+    env_Persistent Δ → Persistent (env_lookup x Δ v).
+  Proof. intros HΔ; revert x; induction HΔ=>-[|?] /=; apply _. Qed.
+  Global Instance interp_persistent τ Δ v :
+    env_Persistent Δ → Persistent (interp τ Δ v).
+  Proof.
+    revert v Δ; induction τ=> v Δ HΔ; simpl; try apply _.
+    rewrite /Persistent fixpoint_interp_rec1_eq /interp_rec1 /= intuitionistically_into_persistently.
+    by apply persistently_intro'.
+  Qed.
+  Global Instance interp_env_base_persistent Δ Γ vs :
+  env_Persistent Δ → TCForall Persistent (zip_with (λ τ, ⟦ τ ⟧ Δ) Γ vs).
+  Proof.
+    intros HΔ. revert vs.
+    induction Γ => vs; simpl; destruct vs; constructor; apply _.
+  Qed.
+  Global Instance interp_env_persistent Γ Δ vs :
+    env_Persistent Δ → Persistent (⟦ Γ ⟧* Δ vs) := _.
+
+  Ltac properness :=
+    repeat match goal with
+    | |- (∃ _: _, _)%I ≡ (∃ _: _, _)%I => apply exist_proper =>?
+    | |- (∀ _: _, _)%I ≡ (∀ _: _, _)%I => apply forall_proper =>?
+    | |- (_ ∧ _)%I ≡ (_ ∧ _)%I => apply and_proper
+    | |- (_ ∨ _)%I ≡ (_ ∨ _)%I => apply or_proper
+    | |- (_ → _)%I ≡ (_ → _)%I => apply impl_proper
+    | |- (WP _ {{ _ }})%I ≡ (WP _ {{ _ }})%I => apply wp_proper =>?
+    | |- (▷ _)%I ≡ (▷ _)%I => apply later_proper
+    | |- (□ _)%I ≡ (□ _)%I => apply intuitionistically_proper
+    | |- (_ ∗ _)%I ≡ (_ ∗ _)%I => apply sep_proper
+    | |- (inv _ _)%I ≡ (inv _ _)%I => apply (contractive_proper _)
+    end.
+  Section Autosubst_Lemmas.
+    Context {term : Type} {Ids_term : Ids term}
+            {Rename_term : Rename term} {Subst_term : Subst term}
+            {SubstLemmas_term : SubstLemmas term}.
+
+    Lemma iter_up (m x : nat) (f : var → term) :
+      upn m f x = if lt_dec x m then ids x else rename (+m) (f (x - m)).
+    Proof.
+      revert x; induction m as [|m IH]=> -[|x];
+        repeat (destruct (lt_dec _ _) || asimpl || rewrite IH); auto with lia.
+    Qed.
+  End Autosubst_Lemmas.
+
+  Lemma interp_weaken Δ1 Π Δ2 τ :
+    ⟦ τ.[upn (length Δ1) (ren (+ length Π))] ⟧ (Δ1 ++ Π ++ Δ2)
+    ≡ ⟦ τ ⟧ (Δ1 ++ Δ2).
+  Proof.
+    revert Δ1 Π Δ2. induction τ=> Δ1 Π Δ2; simpl; auto.
+    - intros w; simpl; properness; auto. by apply IHτ1. by apply IHτ2.
+    - intros w; simpl; properness; auto. by apply IHτ1. by apply IHτ2.
+    - intros w; simpl; properness; auto. by apply IHτ1. by apply IHτ2.
+    - apply fixpoint_proper=> τi w /=.
+      properness; auto. apply (IHτ (_ :: _)).
+    - rewrite iter_up; destruct lt_dec as [Hl | Hl]; simpl.
+      { by rewrite !lookup_app_l. }
+      (* FIXME: Ideally we wouldn't have to do this kinf of surgery. *)
+      change (bi_ofeO (uPredI (iResUR Σ))) with (uPredO (iResUR Σ)).
+      rewrite !lookup_app_r; [|lia ..]. do 2 f_equiv. lia.
+    (* - intros w; simpl; properness; auto. apply (IHτ (_ :: _)). *)
+  Qed.
+
+  Lemma interp_subst_up Δ1 Δ2 τ τ' :
+    ⟦ τ ⟧ (Δ1 ++ interp τ' Δ2 :: Δ2)
+    ≡ ⟦ τ.[upn (length Δ1) (τ' .: ids)] ⟧ (Δ1 ++ Δ2).
+  Proof.
+    revert Δ1 Δ2; induction τ=> Δ1 Δ2; simpl; auto.
+    - intros w; simpl; properness; auto. by apply IHτ1. by apply IHτ2.
+    - intros w; simpl; properness; auto. by apply IHτ1. by apply IHτ2.
+    - intros w; simpl; properness; auto. by apply IHτ1. by apply IHτ2.
+    - apply fixpoint_proper=> τi w /=.
+      properness; auto. apply (IHτ (_ :: _)).
+    - rewrite iter_up; destruct lt_dec as [Hl | Hl]; simpl.
+      { by rewrite !lookup_app_l. }
+      (* FIXME: Ideally we wouldn't have to do this kinf of surgery. *)
+      change (bi_ofeO (uPredI (iResUR Σ))) with (uPredO (iResUR Σ)).
+      rewrite !lookup_app_r; [|lia ..].
+      case EQ: (x - length Δ1) => [|n]; simpl.
+      { symmetry. asimpl. apply (interp_weaken [] Δ1 Δ2 τ'). }
+      change (bi_ofeO (uPredI (iResUR Σ))) with (uPredO (iResUR Σ)).
+      rewrite !lookup_app_r; [|lia ..]. do 2 f_equiv. lia.
+  Qed.
+
+  Lemma interp_subst Δ2 τ τ' v : ⟦ τ ⟧ (⟦ τ' ⟧ Δ2 :: Δ2) v ≡ ⟦ τ.[τ'/] ⟧ Δ2 v.
+  Proof. apply (interp_subst_up []). Qed.
+
+  Lemma interp_env_length Δ Γ vs : ⟦ Γ ⟧* Δ vs ⊢ ⌜length Γ = length vs⌝.
+  Proof. by iIntros "[% ?]". Qed.
+
+  Lemma interp_env_Some_l Δ Γ vs x τ :
+    Γ !! x = Some τ → ⟦ Γ ⟧* Δ vs ⊢ ∃ v, ⌜vs !! x = Some v⌝ ∧ ⟦ τ ⟧ Δ v.
+  Proof.
+    iIntros (?) "[Hlen HΓ]"; iDestruct "Hlen" as %Hlen.
+    destruct (lookup_lt_is_Some_2 vs x) as [v Hv].
+    { by rewrite -Hlen; apply lookup_lt_Some with τ. }
+    iExists v; iSplit. done. iApply (big_sepL_elem_of with "HΓ").
+    apply elem_of_list_lookup_2 with x.
+    rewrite lookup_zip_with; by simplify_option_eq.
+  Qed.
+
+  Lemma interp_env_nil Δ : ⊢ ⟦ [] ⟧* Δ [].
+  Proof. iSplit; simpl; auto. Qed.
+  Lemma interp_env_cons Δ Γ vs τ v :
+    ⟦ τ :: Γ ⟧* Δ (v :: vs) ⊣⊢ ⟦ τ ⟧ Δ v ∗ ⟦ Γ ⟧* Δ vs.
+  Proof.
+    rewrite /interp_env /= (assoc _ (⟦ _ ⟧ _ _)) -(comm _ ⌜(_ = _)⌝%I) -assoc.
+    by apply sep_proper; [apply pure_proper; lia|].
+  Qed.
+
+  Lemma interp_env_ren Δ (Γ : list type) (vs : list val) τi :
+    ⟦ subst (ren (+1)) <$> Γ ⟧* (τi :: Δ) vs ⊣⊢ ⟦ Γ ⟧* Δ vs.
+  Proof.
+    apply sep_proper; [apply pure_proper; by rewrite fmap_length|].
+    revert Δ vs τi; induction Γ=> Δ [|v vs] τi; csimpl; auto.
+    apply sep_proper; auto. apply (interp_weaken [] [τi] Δ).
+  Qed.
 End logrel.
 
+Typeclasses Opaque interp_env.
 Notation "⟦ τ ⟧" := (interp τ).
 Notation "⟦ τ ⟧ₑ" := (interp_expr τ).
 Notation "⟦ Γ ⟧*" := (interp_env Γ).
